Setlec/Verify/InferLeaves.lean
@@ -539,7 +539,7 @@ theorem whnfPres_fvarLeaves {env : Env} (henv : EnvWF env) :
             cases this
         simp only [fvarLeaves]
         rcases hcase with rfl |
-          ⟨us, entry, hfn, hf, hnat, hi, hlen, hus, hred, -, -⟩
+          ⟨us, entry, hfn, hf, hnat, hi, hlen, hus, hred, -⟩
         · simp only [fvarLeaves] at hl
           exact ihLoop he l (hsub₃ l hl)
         · have hl2 := ihCore hred l hl
@@ -668,7 +668,7 @@ theorem whnfPres_looseBVars {env : Env} (henv : EnvWF env) :
           · exact hbe₂
           · exact ihLoop hred (strLitToConstructor_looseBVars s 0)
         rcases hcase with rfl |
-          ⟨us, entry, hfn, hf, hnat, hi, hlen, hus, hred, -, -⟩
+          ⟨us, entry, hfn, hf, hnat, hi, hlen, hus, hred, -⟩
         · simpa [looseBVarsBounded] using hbe₃
         · exact ihCore hred
             (looseBVarsBounded_getAppArgs hbe₃ _ (getD_mem (by omega)))
@@ -812,7 +812,7 @@ theorem inferTypeCore_WScoped {env : Env} (henv : EnvWF env) :
       exact WScoped.instantiate1_gen hw.2 0 hwPi.2
     | proj sn i pe =>
       obtain ⟨tpe, te, T, us, entry, hte, hwt, hfn, hfp, hnat, hlen,
-        hus, -, hres⟩ := inferTypeCore_proj_inv h
+        hus, hres⟩ := inferTypeCore_proj_inv h
       simp only [WScoped] at hw
       have hwte := inferTypeCore_WScoped henv fuel hte hw
       have hwPi := whnf_WScoped henv fuel hwt hwte
@@ -945,7 +945,7 @@ theorem inferTypeCore_fvarLeaves {env : Env} (henv : EnvWF env) :
       · exact Or.inr hb
     | proj sn i pe =>
       obtain ⟨tpe, te, T, us, entry, hte, hwt, hfn, hfp, hnat, hlen,
-        hus, -, hres⟩ := inferTypeCore_proj_inv h
+        hus, hres⟩ := inferTypeCore_proj_inv h
       simp only [WScoped] at hw
       intro l hl
       simp only [fvarLeaves]
@@ -1083,7 +1083,7 @@ theorem inferTypeCore_looseBVars {env : Env} (henv : EnvWF env) :
       exact looseBVarsBounded_instantiate1_gen hb.2 hbPi.2
     | proj sn i pe =>
       obtain ⟨tpe, te, T, us, entry, hte, hwt, hfn, hfp, hnat, hlen,
-        hus, -, hres⟩ := inferTypeCore_proj_inv h
+        hus, hres⟩ := inferTypeCore_proj_inv h
       simp only [WScoped] at hw
       simp only [looseBVarsBounded] at hb
       have hLbe : Expr.LeavesBounded pe := fun l hl => hLb l (by
